SSA/Projects/InstCombine/Tactic.lean
@@ -2,9 +2,11 @@ import SSA.Projects.InstCombine.LLVM.EDSL
 import SSA.Projects.InstCombine.AliveStatements
 import SSA.Projects.InstCombine.Refinement
 import Mathlib.Tactic
+import SSA.Core.ErasedContext
 
 open MLIR AST
 open Std (BitVec)
+open Ctxt
 
 theorem bitvec_minus_one : BitVec.ofInt w (Int.negSucc 0) = (-1 : BitVec w) := by
   simp[BitVec.ofInt, BitVec.ofNat,Neg.neg,
@@ -19,6 +21,8 @@ theorem bitvec_minus_one : BitVec.ofInt w (Int.negSucc 0) = (-1 : BitVec w) := b
       simp
     rw[ONE]
 
+
+open MLIR AST in
 /--
 - We first simplify `Com.refinement` to see the context `Γv`.
 - We `simp_peephole Γv` to simplify context accesses by variables.
@@ -34,14 +38,14 @@ macro "simp_alive_peephole" : tactic =>
         intros Γv
         simp [InstcombineTransformDialect.MOp.instantiateCom, InstcombineTransformDialect.instantiateMOp,
           ConcreteOrMVar.instantiate, Vector.get, List.nthLe, List.length_singleton, Fin.coe_fin_one, Fin.zero_eta,
-          List.get_cons_zero, Function.comp_apply, InstcombineTransformDialect.instantiateMTy, Ctxt.empty_eq, DerivedCtxt.snoc,
-          DerivedCtxt.ofCtxt, List.map_eq_map, List.map] at Γv
-        simp_peephole at Γv
+          List.get_cons_zero, Function.comp_apply, InstcombineTransformDialect.instantiateMTy, Ctxt.empty_eq, Ctxt.DerivedCtxt.snoc,
+          Ctxt.DerivedCtxt.ofCtxt, List.map_eq_map, List.map, DialectMorphism.mapTy] at Γv
+        simp_peephole_mlir at Γv
         /- note that we need the `HVector.toPair`, `HVector.toSingle`, `HVector.toTriple` lemmas since it's used in `InstCombine.Op.denote`
           We need `HVector.toTuple` since it's used in `MLIR.AST.mkOpExpr`. -/
-        try simp (config := {decide := false}) only [OpDenote.denote,
+        simp (config := {decide := false}) only [OpDenote.denote,
           InstCombine.Op.denote, HVector.toPair, HVector.toTriple, pairMapM, BitVec.Refinement,
-          bind, Option.bind, pure, DerivedCtxt.ofCtxt, DerivedCtxt.snoc,
+          bind, Option.bind, pure, Ctxt.DerivedCtxt.ofCtxt, Ctxt.DerivedCtxt.snoc,
           Ctxt.snoc,
           ConcreteOrMVar.instantiate, Vector.get, HVector.toSingle,
           LLVM.and?, LLVM.or?, LLVM.xor?, LLVM.add?, LLVM.sub?,
@@ -54,7 +58,8 @@ macro "simp_alive_peephole" : tactic =>
           InstcombineTransformDialect.instantiateMOp,
           InstcombineTransformDialect.MOp.instantiateCom,
           InstcombineTransformDialect.instantiateCtxt,
-          ConcreteOrMVar.instantiate, Com.Refinement]
+          ConcreteOrMVar.instantiate, Com.Refinement,
+          DialectMorphism.mapTy]
         try intros v0
         try intros v1
         try intros v2
